dataset/filesystems/interface/effectful-interface.dfy
@@ -3,49 +3,63 @@ newtype{:nativeType "byte"} byte = i:int | 0 <= i < 0x100
 newtype{:nativeType "int"} int32 = i:int | -0x80000000 <= i < 0x80000000
 newtype{:nativeType "int"} nat32 = i:int | 0 <= i < 0x80000000
 newtype{:nativeType "int"} maxPath = i:int | 0 <= i < 256
-datatype path = path(length: int, data: seq<char>) //datatype image = image(width: int, height: int, data: seq<byte>)
-datatype access = access(accessType: seq<char>)
+// datatype path = path(length: int, data: seq<char>) //datatype image = image(width: int, height: int, data: seq<byte>)
+// datatype access = access(accessType: seq<char>)
 type NonEmptySeq = x: seq<char> | |x| > 0 witness ['a']
+// Define a type for file system entries
+datatype FSEntry = File(content: seq<byte>) | Directory(entries: map<string, FSEntry>)
+
 // newtype{:nativeType "char"} validPathChar = c:char | c
 // newtype{:nativeType "path"} path = c:char | 
 
-//TODO: Should avoid data races (reading and writing data at the same time)
+//TODO: Avoid data races (reading and writing data at the same time)
 
-// class OkState
+// class ReadWriteLock {
+//   var readers: nat
+//   var writer: bool
+
+//   constructor()
+//     ensures readers == 0 && !writer
 //   {
-//   // constructor{:axiom} () requires false // unconstructible during real execution
-//    constructor() {}
-//   function{:axiom} ok():bool reads this // reads the state of okState and returns a boolean
-// }
-// class OkState {
-//   var isOk: bool;
-
-//   constructor() {
-//     isOk := true;
+//     readers := 0;
+//     writer := false;
 //   }
 
-//   method UpdateOk(newState: bool)
+//   method acquireRead()
 //     modifies this
-//     ensures isOk == newState
+//     ensures old(readers) < readers
+//     ensures !writer
 //   {
-//     isOk := newState;
+//     assume !writer;
+//     readers := readers + 1;
 //   }
 
-//   predicate{:axiom} ok()
-//     reads this
+//   method releaseRead()
+//     modifies this
+//     requires readers > 0
+//     ensures readers == old(readers) - 1
 //   {
-//     isOk
+//     readers := readers - 1;
+//   }
+
+//   method acquireWrite()
+//     modifies this
+//     ensures writer
+//     ensures readers == 0
+//   {
+
+//     assume readers == 0 && !writer;
+//     writer := true;
+//   }
+
+//   method releaseWrite()
+//     modifies this
+//     requires writer
+//     ensures !writer
+//   {
+//     writer := false;
 //   }
 // }
-// class HostEnvironment
-//   {
-//   var ok:OkState
-//   // constructor{:axiom} () requires false // non-constructive
-//   constructor() {
-//     ok := new OkState();
-//   }
-//   // ghost var ok:OkState // only for specificaions and verifications with no run-time effect
-//  }
 
 class OkState
   {
@@ -60,31 +74,43 @@ class HostEnvironment
 }
 
 
-
 class FileStream
   {
   var env:HostEnvironment
+  // The file system is a map from paths to FSEntries
+  var fs: map<path, FSEntry>
+  // var locks: map<path, ReadWriteLock>
+  var currentDirectory: path
   function{:axiom} Name():string reads this
   function{:axiom} IsOpen():bool reads this
   constructor{:axiom} () requires false
-  // function{:axiom} Access():string reads this
-  // function {:axiom} Capabilities():(string, string) reads this
-  // function{:axiom} Path():string reads this
+
+  // Helper predicate to check if a path is a directory
+  predicate isDirectory(p: path)
+    reads this
+  {
+    p in fs.Keys && fs[p].Directory?
+  }
+
+  // Helper function to get the contents of a directory
+  function getDirectoryContents(p: path): map<string, FSEntry>
+    requires isDirectory(p)
+    reads this
+  {
+    match fs[p] {
+      case Directory(entries) => entries
+      case File(_) => map[] // This case should never occur due to the requires clause
+    }
+  }
 
 
   // static method{:axiom} Open(name:array<char>, ghost env:HostEnvironment, access:array<char>)
-  static method{:axiom} Open(name:seq<char>, env:HostEnvironment)
+  static method{:axiom} Open(name: path)
     returns(ok:bool, f:FileStream)
     requires name[..] in nonSensitiveFilesList
     requires name[..] !in sensitivePaths
     requires validate_file(name)
-    // filetype validation should be done here
-    // requires access[..] in ["read", "write"]
-    // requires capabilities in [("bar.txt", "write")]
-    requires env.ok.ok()
-    modifies env.ok
-    ensures  env.ok.ok() == ok
-    ensures  ok ==> fresh(f) && f.env == env && f.IsOpen() && f.Name() == name[..]
+    ensures  ok ==> fresh(f) && f.IsOpen() && f.Name() == name[..]
     ensures f.IsOpen() <==> validate_file(name)
 
 
@@ -95,113 +121,108 @@ class FileStream
     requires env.ok.ok()
     requires IsOpen()
     modifies this
-    modifies env.ok
-    ensures  env == old(env)
-    ensures  env.ok.ok() == ok
 
-  method{:axiom} Read(fileOffset:nat32, buffer:array<byte>, start:int32, end:int32) returns(ok:bool)
-    requires env.ok.ok()
+  method{:axiom} Read(f: file, fileOffset:nat32, buffer:array<byte>, start:int32, end:int32) returns(ok:bool)
+    // modifies this`locks
+    modifies this
     requires IsOpen()
     requires 0 <= start as int <= end as int <= buffer.Length
-    requires Name() in nonSensitiveFilesList
-    requires Name() !in sensitivePaths
+    requires 0 < |f| <= fileMaxLength
+    requires 0 < |f| - 4 <= 10 //checks file type exists 
+    //ToDo: validation file type format is required .txt, .pdf, .docx
+    requires contains_sequence(nonSensitiveFilesList, f)
+    requires f !in sensitivePaths
+    requires f[(|f| - 4)..] !in invalidFileTypes
     // requires Access() in ["read", "write"]
     // requires Capabilities() in [("bar.txt", ["read, write"]), ("baz.txt", ["read"])]
-    modifies env.ok
     modifies buffer
-    ensures  env == old(env)
-    ensures  env.ok.ok() == ok
     ensures  Name() == old(Name())
     ensures  forall i:int :: 0 <= i < buffer.Length && !(start as int <= i < end as int) ==> buffer[i] == old(buffer[i])
     ensures  ok ==> IsOpen()
+    ensures ok <==> validate_file_type(f)
 
-  method{:axiom} Write(fileName: seq<char>, fileOffset:nat32, buffer:array<byte>, start:int32, end:int32) returns(ok:bool)
+   
+  method{:axiom} Write(f: file, fileOffset:nat32, buffer:array<byte>, start:int32, end:int32) returns(ok:bool)
   // method{:axiom} Write(fileOffset:nat32, buffer:seq<byte>, start:int32, end:int32) returns(ok:bool)
-    requires env.ok.ok()
     requires IsOpen()
     requires 0 <= start as int <= end as int <= buffer.Length
     // requires 0 <= start as int <= end as int <= |buffer|
-    requires Name() in nonSensitiveFilesList
-    requires 0 < |fileName| <= fileMaxLength
-    requires 0 < |fileName| - 4 <= 10 //checks file type exists 
+    requires f in nonSensitiveFilesList
+    requires 0 < |f| <= fileMaxLength
+    requires 0 < |f| - 4 <= 10 //checks file type exists 
     //ToDo: validation file type format is required .txt, .pdf, .docx
-    requires contains_sequence(nonSensitiveFilesList, fileName)
-    requires fileName !in sensitivePaths
-    requires fileName[(|fileName| - 4)..] !in invalidFileTypes
+    requires contains_sequence(nonSensitiveFilesList, f)
+    requires f !in sensitivePaths
+    requires f[(|f| - 4)..] !in invalidFileTypes
     // requires Access() in ["read", "write"]
     // requires Capabilities in [("bar.txt", ["read, write"]), ("baz.txt", ["read"])]
     modifies this
-    modifies env.ok
-    ensures  env == old(env)
-    ensures  env.ok.ok() == ok
     ensures  Name() == old(Name())
     ensures  ok ==> IsOpen()
 
   method{:axiom} Flush() returns(ok:bool)
-    requires env.ok.ok()
     requires IsOpen()
     modifies this
-    modifies env.ok
-    ensures  env == old(env)
-    ensures  env.ok.ok() == ok
     ensures  Name() == old(Name())
     ensures  ok ==> IsOpen()
 
-
-  method{:axiom} IsValidDirectoryName(dirName: seq<char>) // should not be axioms
-    // Check if the directory name is not empty
-    requires 0 < |dirName| <= dirMaxLength 
-    // Check if each character in the directory name is a valid character
-    ensures forall i :: 0 <= i < |dirName| ==> validate_file_char(dirName[i])  
-    
-
-  method{:axiom} Join(path:seq<char>, fileName:seq<char>) returns(ok:bool, result:seq<char>)
-    requires 0 < |fileName| <= fileMaxLength
-    requires 0 < |path| <= dirMaxLength - fileMaxLength
-    requires contains_sequence(nonSensitiveFilesList, fileName)
-    requires path !in sensitivePaths
-    requires path in currWDir && validate_dir_name(path)
-    requires fileName in nonSensitiveFilesList && Name() in nonSensitiveFilesList
-    requires fileName[(|fileName| - 4)..] !in invalidFileTypes
-    requires |path| > 0 // ToDo: Use a function for path validation
-    requires env.ok.ok()
-    requires has_absolute_path(path) && path[..] !in sensitivePaths
+  method{:axiom} Join(p: path, f: file) returns(ok:bool, result: path)
+    requires 0 < |f| <= fileMaxLength
+    requires 0 < |p| <= dirMaxLength - fileMaxLength - 1
+    requires contains_sequence(nonSensitiveFilesList, f)
+    requires p !in sensitivePaths
+    requires validate_dir_name(p)
+    requires f in nonSensitiveFilesList && Name() in nonSensitiveFilesList
+    requires f[(|f| - 4)..] !in invalidFileTypes
+    requires |p| > 0 // ToDo: Use a function for path validation
+    requires has_absolute_path(p) && p[..] !in sensitivePaths
     requires IsOpen()
     modifies this
-    modifies env.ok
-    ensures  env != old(env)
-    ensures  env.ok.ok() == ok
     ensures  Name() == old(Name())
-    ensures result == path_join(path, fileName)
+    ensures result == path_join(p, f)
     ensures has_absolute_path(result) && result[..] !in sensitivePaths
-    ensures  ok ==> path_join(path, fileName) == result && has_absolute_path(result) && result[..] !in sensitivePaths
+    ensures  ok ==> path_join(p, f) == result && has_absolute_path(result) && result[..] !in sensitivePaths
 
-  method{:axiom} GetCWD(currDir: seq<char>) returns (ok: bool)
-  modifies this
-  modifies env.ok
-  requires env.ok.ok()
-  requires currDir !in sensitivePaths
-  requires currDir in currWDir
-  ensures  env == old(env)
-  ensures  env.ok.ok() == ok
-  ensures  Name() == old(Name())
-
-  method{:axiom} rmdir (dirname: seq<char>) returns (ok:bool)
+  method{:axiom} GetCurrentDirectory() returns (cwd: path)
+    // Method to get the current working directory
     modifies this
-    modifies env.ok
-    requires env.ok.ok()
-    requires dirname !in sensitivePaths
-    ensures  env == old(env)
-    ensures  env.ok.ok() == ok
+    ensures cwd !in sensitivePaths
+    ensures cwd == currentDirectory
+    ensures cwd in fs.Keys && fs[cwd].Directory?
+  
+
+  method{:axiom} remove (dir: path) returns (success: bool)
+    requires |dir| <= dirMaxLength  // The path must be valid
+    requires dir !in sensitivePaths
+    modifies this
+    requires dir in fs.Keys  // The directory must exist
+    requires validate_dir_name(dir)  // The path must point to a directory
+    requires isDirectory(dir)
+    requires forall p | p in fs.Keys :: !isPrefix(dir, p) || p == dir  // The directory must be empty
+    modifies this
+    ensures old(dir in fs.Keys) && !success ==>
+              fs == old(fs)  // If removal fails, the file system is unchanged
+    ensures success ==>
+              fs == map p | p in old(fs.Keys) && p != dir :: old(fs[p])  // If successful, dir is removed
+    ensures old(dir in fs.Keys) ==> success  // If the directory existed, removal should succeed
     ensures  Name() == old(Name())
+
+  //     // Method to change the current working directory
+  // method changeDirectory(newDir: path) returns (success: bool)
+  //   requires newDir in fs.Keys
+  //   modifies this
+  //   ensures success ==> currentDirectory == newDir && fs[newDir].Directory?
+  //   ensures !success ==> currentDirectory == old(currentDirectory)
+  // {
+  //   if newDir in fs.Keys && fs[newDir].Directory? {
+  //     currentDirectory := newDir;
+  //     success := true;
+  //   } else {
+  //     success := false;
+  //   }
+  // }
+
 
 // TODO: How to link axioms to python functions
-// TODO: Basically Join is similar to concatenation of two string
-  // method concatenation(str1: seq<char>, str2: seq<char>) returns (ok: bool, result: seq<char>) 
-  // requires env.ok.ok()
-  // modifies this
-  // modifies env.ok
-  // ensures  env == old(env)
-  // ensures  env.ok.ok() == ok
 
 }
