dataset/filesystems/interface/interface-helper.dfy
@@ -1,17 +1,21 @@
-const dirMaxLength := 4096
-const fileMaxLength := 255
-const fileMinLength := 4
+type path = seq<char>
+type file = seq<char>
+type fileType = seq<char>
+const dirMaxLength :int  := 4096
+const fileMaxLength :int := 255
+const fileMinLength :int := 4
 const validFileCharacters := {'.', '-'}
 const validDirCharacters := {'_', '.', '-', '/'}
 
 // Constants for sensitive paths and files
 const invalidFileTypes :=  [".php", "CON", "PRN", "AUX", "NUL", "COM1", "COM2", "COM3", "COM4", "LPT1", "LPT2", "LPT3", "LPT4", "LPT5", "LPT6", "LPT7", "LPT8", "LPT9"]
-const sensitivePaths := ["/usr", "/System", "/bin", "/sbin", "/var", "/usr/local"]
+const sensitivePaths := ["/usr", "/System", "/bin", "/sbin", "/var", "/usr/local", "/documnets"]
 const currWDir := ["/Users/pari/pcc-llms/src/playground"]
-const nonSensitiveFilesList := ["public-key.txt", "safeFile-1.txt", "safeFile-2.txt", "safeFile-3.txt", "bar.txt", "baz.txt"]
-// TODO: Define a new datatype for path (os.path type is a string)
-// TODO: Add constant values for CWD and everytime get.cwd is called it should check the value be the same
-
+const nonSensitiveFilesList : seq<seq<char>> := ["public-key.txt", "safeFile-1.txt", "safeFile-2.txt", "safeFile-3.txt", "bar.txt", "baz.txt"]
+ // Set of allowed file extensions
+const allowedExtensionsForRead: seq<string> := ["txt", "pdf", "docx"]
+datatype Permission = Read | Write | Execute
+type User = seq<char>
 
 predicate alpha_numeric(c: char)
 
@@ -39,7 +43,7 @@ ensures validate_dir_char(c) <==> alpha_numeric(c) || c in validDirCharacters
     alpha_numeric(c) || c in validDirCharacters
 }
 
-method ValidateNonsensitiveFile(fileName: seq<char>, nonSensitiveFilesList: seq<seq<char>>) returns (result: bool)
+method ValidateNonsensitiveFile(fileName: file, nonSensitiveFilesList: seq<path>) returns (result: bool)
 requires 0 < |fileName| <= fileMaxLength
 ensures result <==> (exists i :: 0 <= i < |nonSensitiveFilesList| && fileName == nonSensitiveFilesList[i]) || fileName in nonSensitiveFilesList
 {
@@ -74,64 +78,104 @@ ensures |concat(s1, s2)| == |s1| + |s2| && concat(s1, s2) == s1 + s2 && |s1| + |
   s1 + s2
 }
 
-function path_join(s1: seq<char>, s2: seq<char>): seq<char>
-requires 0 <= |s1| + |s2| && 0 < |s1| <= dirMaxLength - fileMaxLength - 1 && 0 < |s2| <= fileMaxLength
-ensures |concat(concat(s1, "/"), s2)| == |s1| + |s2| + 1 && concat(concat(s1, "/"), s2) == s1 + "/" + s2 && |s1| + |s2| <= dirMaxLength 
+function path_join(p: path, f: file): seq<char>
+requires 0 <= |p| + |f| && 0 < |p| <= dirMaxLength - fileMaxLength - 1 && 0 < |f| <= fileMaxLength
+ensures |concat(concat(p, "/"), f)| == |p| + |f| + 1 && 
+        concat(concat(p, "/"), f) == p + "/" + f && |p| + |f| <= dirMaxLength 
 {
-  if s1[|s1| - 1] == '/' then  concat(s1, s2) else concat(concat(s1, "/"), s2)
+  if p[|p| - 1] == '/' then  concat(p, f) else concat(concat(p, "/"), f)
 }
 
 
-predicate has_path_traversal(s: seq<char>)
-ensures has_path_traversal(s) <==> exists i :: 0 <= i < |s| && is_traversal_pattern(s, i)
+predicate has_path_traversal(p: path)
+ensures has_path_traversal(p) <==> exists i :: 0 <= i < |p| && is_traversal_pattern(p, i)
 {
-    exists i :: 0 <= i < |s| && is_traversal_pattern(s, i)
+    exists i :: 0 <= i < |p| && is_traversal_pattern(p, i)
 }
 
-predicate is_traversal_pattern(s: seq<char>, i: int)
-requires 0 <= i < |s|
+predicate is_traversal_pattern(p: path, i: int)
+requires 0 <= i < |p|
 {
-    (i + 2 < |s| && s[i] == '.' && s[i+1] == '.' && (s[i+2] == '/' || s[i+2] == '\\')) ||
-    (i + 5 < |s| && s[i..i+6] == ['%', '2', 'e', '%', '2', 'e']) ||
-    (i + 8 < |s| && s[i..i+9] == ['%', '2', '5', '2', 'e', '%', '2', '5', '2', 'e']) ||
-    (i > 0 && s[i-1] == '/' && i + 2 < |s| && s[i] == '.' && s[i+1] == '.' && s[i+2] == '.')
+    (i + 2 < |p| && p[i] == '.' && p[i+1] == '.' && (p[i+2] == '/' || p[i+2] == '\\')) ||
+    (i + 5 < |p| && p[i..i+6] == ['%', '2', 'e', '%', '2', 'e']) ||
+    (i + 8 < |p| && p[i..i+9] == ['%', '2', '5', '2', 'e', '%', '2', '5', '2', 'e']) ||
+    (i > 0 && p[i-1] == '/' && i + 2 < |p| && p[i] == '.' && p[i+1] == '.' && p[i+2] == '.')
 }
 
-predicate is_dangerous_path(s: seq<char>)
-ensures is_dangerous_path(s) <==> has_path_traversal(s) || has_absolute_path(s)
+predicate is_dangerous_path(p: path)
+ensures is_dangerous_path(p) <==> has_path_traversal(p) || has_absolute_path(p)
 {
-    has_path_traversal(s) || has_absolute_path(s)
+    has_path_traversal(p) || has_absolute_path(p)
 }
 
-predicate has_absolute_path(s: seq<char>)
-ensures has_absolute_path(s) <==> |s| > 0 && (s[0] == '/' || (|s| > 1 && s[1] == ':'))
+predicate has_absolute_path(p: path)
+ensures has_absolute_path(p) <==> |p| > 0 && (p[0] == '/' || (|p| > 1 && p[1] == ':'))
 {
-    |s| > 0 && (s[0] == '/' || (|s| > 1 && s[1] == ':'))
-}
-
-
-
-predicate validate_file(fileName: seq<char>)
-requires 0 <= |fileName| <= fileMaxLength
-ensures validate_file(fileName) <==> forall i :: 0 <= i < |fileName|  ==> validate_file_char(fileName[i]) && alpha_numeric(fileName[0]) && alpha_numeric(fileName[|fileName| - 1])
-{
-  forall i :: 0 <= i < |fileName| ==> validate_file_char(fileName[i]) && alpha_numeric(fileName[0]) && alpha_numeric(fileName[|fileName| - 1])
-
+    |p| > 0 && (p[0] == '/' || (|p| > 1 && p[1] == ':'))
 }
 
 
 
-predicate validate_dir_name(dirName: seq<char>)
-requires 0 <= |dirName| <= dirMaxLength
-  ensures validate_dir_name(dirName) <==> forall i :: 0 <= i < |dirName| ==> validate_char(dirName[i])
+predicate validate_file(f: file)
+requires 0 <= |f| <= fileMaxLength
+ensures validate_file(f) <==> (forall i :: 0 <= i < |f|  ==> validate_file_char(f[i])
+         && alpha_numeric(f[0]) && alpha_numeric(f[|f| - 1]))
 {
-  forall i :: 0 <= i < |dirName| ==> validate_char(dirName[i])
+  forall i :: 0 <= i < |f| ==> validate_file_char(f[i]) && alpha_numeric(f[0]) && alpha_numeric(f[|f| - 1])
+
 }
 
-method ValidateFileType(fileType: seq<char>) returns (result: bool)
-requires 0 <= |fileType| <= 4
+
+
+predicate validate_dir_name(p: path)
+requires 0 <= |p| <= dirMaxLength
+  ensures validate_dir_name(p) <==> forall i :: 0 <= i < |p| ==> validate_char(p[i])
 {
-  var res := ContainsSequence(nonSensitiveFilesList, fileType);
+  forall i :: 0 <= i < |p| ==> validate_char(p[i])
+}
+
+predicate validate_file_type(f: file)
+  ensures validate_file_type(f) <==> (getFileExtension(f) in allowedExtensionsForRead
+   && getFileExtension(f) !in invalidFileTypes)
+{
+  var extension := getFileExtension(f);
+  if (extension in allowedExtensionsForRead  && extension !in invalidFileTypes) then true else false
+}
+
+// Helper function to get the last index of a character in a sequence
+function lastIndexOf(s: seq<char>, c: char): int
+  ensures -1 <= lastIndexOf(s, c) < |s|
+  ensures lastIndexOf(s, c) != -1 ==> s[lastIndexOf(s, c)] == c
+  ensures forall i :: lastIndexOf(s, c) < i < |s| ==> s[i] != c
+{
+  if |s| == 0 then -1
+  else if s[|s|-1] == c then |s| - 1
+  else lastIndexOf(s[..|s|-1], c)
+}
+
+// Helper function to get file extension
+function getFileExtension(filename: file): string
+{
+    var lastDotIndex := lastIndexOf(filename, '.');
+    if lastDotIndex == -1 then
+      []
+    else
+      filename[lastDotIndex + 1..]
+}
+
+//  predicate hasPathPermission(path: path, user: User, perm: Permission)
+//  ensures hasPathPermission(path, user, perm) <==> path in permissions.Keys && user in permissions[path].Keys && perm in permissions[path][user]
+//   {
+//     && path in permissions.Keys
+//     && user in permissions[path].Keys
+//     && perm in permissions[path][user]
+//   }
+
+
+method ValidateFileType(t: fileType) returns (result: bool)
+requires 0 <= |t| <= 4
+{
+  var res := ContainsSequence(nonSensitiveFilesList, t);
   if !res {
     result := true;
   } else {
@@ -159,6 +203,12 @@ method ContainsC(s: string, c: char) returns (result: bool)
 
   }
 
+}
+
+
+predicate isPrefix(p1: path, p2: path)
+{
+  |p1| <= |p2| && p1 == p2[..|p1|]
 }
 
 method ContainsSequence(list: seq<seq<char>>, sub: seq<char>) returns (result: bool)
@@ -275,7 +325,7 @@ function char_to_byte(c: char): int
 }
 
 
-method StringToBytes(s: string) returns (bytesSeq: seq<int>)
+method StringToSeqInt(s: string) returns (bytesSeq: seq<int>)
 // Convert a string to a sequence of bytes<int>
   requires |s| > 0  // Precondition requires non-empty strings
   ensures |s| == |bytesSeq|  //  // Postcondition ensure the length of the generated sequence matches the input string length
@@ -293,6 +343,7 @@ method StringToBytes(s: string) returns (bytesSeq: seq<int>)
   }
 
 }
+
 function contains_sequence(list: seq<seq<char>>, sub: seq<char>): bool
   ensures contains_sequence(list, sub) <==> (exists i :: 0 <= i < |list| && sub == list[i])
 {
