dataset/cwe-samples/task_id_1.dfy
@@ -1,0 +1,14 @@
+include "/Users/pari/pcc-llms/dataset/filesystems/interface/effectful-interface.dfy"
+method SafeJoin(path: seq<char>,  fname: seq<char>) returns (jointPath: path)
+{
+  var fname := "public-key.txt";
+  var f: FileStream;
+  var ok: bool;
+  ok, f := FileStream.Open(fname);
+  if !ok { print "open failed\n"; return "";}
+  var path := "/documents";
+  var joinIsOk:bool;
+  assert fname == "public-key.txt";
+  joinIsOk, jointPath := f.Join(path, fname);
+  assert jointPath == "/documents/public-key.txt";
+}
