dataset/cwe-samples/task_id_2.dfy
@@ -1,0 +1,15 @@
+include "/Users/pari/pcc-llms/dataset/filesystems/interface/effectful-interface.dfy"
+method SafeWrite(fname: seq<char>)
+{
+    var fname := "safeFile-1.txt";
+    var f: FileStream;
+    var ok: bool;
+    ok, f := FileStream.Open(fname);
+    if !ok { print "open failed\n"; return; }
+    // This is "hello world!" in ascii.
+    // The library requires the data to be an array of bytes, but Dafny has no char->byte conversions
+    var data: array<byte> := ArrayFromSeq([104, 101, 108, 108, 111, 32, 119, 111, 114, 108, 100, 33, 10]);
+    ok := f.Write(fname, 0, data, 0, data.Length as int32);
+    print "Safe write operation!\n";
+
+}
