dataset/cwe-samples/task_id_3.dfy
@@ -1,0 +1,17 @@
+include "/Users/pari/pcc-llms/dataset/filesystems/interface/effectful-interface.dfy"
+method SafeRead(fname: seq<char>)
+// Prevents user from reading sensitive files or files without permission
+// Read with checking user permissions for reading the file
+
+{
+    var fname := "safeFile-1.txt";
+    var f: FileStream;
+    var ok: bool;
+    ok, f := FileStream.Open(fname);
+    var user := "admin";
+    if !ok { print "open failed\n"; return; }
+    var data: array<byte> := new byte[100];
+    ok := f.Read(fname, 0, data, 0, data.Length as int32);
+    print "Safe Read operation!\n";
+
+}
